theories/Interp/HandlerFacts.v
@@ -26,7 +26,7 @@ Open Scope itree_scope.
 (* end hide *)
 
 Lemma eh_cmp_id_left_strong {A R} (t : itree A R)
-  : interp (id_ A) R t ≈ t.
+  : interp (id_ A) t ≈ t.
 Proof.
   revert t. ucofix CIH. red. ucofix CIH'. intros.
   rewrite unfold_interp. unfold _interp. repeat red.
